Updates.

HandbookOfPracticalLogicLean/Chapter2.lean
@@ -1293,6 +1293,9 @@ def Formula_.is_nnf :
   | _ => False
 
 
+-------------------------------------------------------------------------------
+
+
 mutual
 def to_nnf_v1 :
   Formula_ → Formula_
@@ -1473,49 +1476,49 @@ example
 
 
 mutual
-def to_nnf :
+def to_nnf_v2 :
   Formula_ → Formula_
-  | not_ phi => to_nnf_neg phi
-  | and_ phi psi => and_ (to_nnf phi) (to_nnf psi)
-  | or_ phi psi => or_ (to_nnf phi) (to_nnf psi)
-  | imp_ phi psi => or_ (to_nnf_neg phi) (to_nnf psi)
-  | iff_ phi psi => or_ (and_ (to_nnf phi) (to_nnf psi)) (and_ (to_nnf_neg phi) (to_nnf_neg psi))
+  | not_ phi => to_nnf_neg_v2 phi
+  | and_ phi psi => and_ (to_nnf_v2 phi) (to_nnf_v2 psi)
+  | or_ phi psi => or_ (to_nnf_v2 phi) (to_nnf_v2 psi)
+  | imp_ phi psi => or_ (to_nnf_neg_v2 phi) (to_nnf_v2 psi)
+  | iff_ phi psi => or_ (and_ (to_nnf_v2 phi) (to_nnf_v2 psi)) (and_ (to_nnf_neg_v2 phi) (to_nnf_neg_v2 psi))
   | phi => phi
 
-def to_nnf_neg :
+def to_nnf_neg_v2 :
   Formula_ → Formula_
-  | not_ phi => to_nnf phi
-  | and_ phi psi => or_ (to_nnf_neg phi) (to_nnf_neg psi)
-  | or_ phi psi => and_ (to_nnf_neg phi) (to_nnf_neg psi)
-  | imp_ phi psi => and_ (to_nnf phi) (to_nnf_neg psi)
-  | iff_ phi psi => or_ (and_ (to_nnf phi) (to_nnf_neg psi)) (and_ (to_nnf_neg phi) (to_nnf psi))
+  | not_ phi => to_nnf_v2 phi
+  | and_ phi psi => or_ (to_nnf_neg_v2 phi) (to_nnf_neg_v2 psi)
+  | or_ phi psi => and_ (to_nnf_neg_v2 phi) (to_nnf_neg_v2 psi)
+  | imp_ phi psi => and_ (to_nnf_v2 phi) (to_nnf_neg_v2 psi)
+  | iff_ phi psi => or_ (and_ (to_nnf_v2 phi) (to_nnf_neg_v2 psi)) (and_ (to_nnf_neg_v2 phi) (to_nnf_v2 psi))
   | phi => not_ phi
 end
 
-#eval to_nnf false_
-#eval to_nnf (not_ false_)
-#eval to_nnf (not_ (not_ false_))
-#eval to_nnf (not_ (not_ (not_ false_)))
-#eval to_nnf (not_ (not_ (not_ (not_ false_))))
+#eval to_nnf_v2 false_
+#eval to_nnf_v2 (not_ false_)
+#eval to_nnf_v2 (not_ (not_ false_))
+#eval to_nnf_v2 (not_ (not_ (not_ false_)))
+#eval to_nnf_v2 (not_ (not_ (not_ (not_ false_))))
 
 
-theorem eval_to_nnf_neg_iff_not_eval_to_nnf
+theorem eval_to_nnf_neg_iff_not_eval_to_nnf_v2
   (V : PropValuation)
   (F : Formula_) :
-  eval V (to_nnf_neg F) ↔ ¬ eval V (to_nnf F) :=
+  eval V (to_nnf_neg_v2 F) ↔ ¬ eval V (to_nnf_v2 F) :=
   by
   induction F
   case false_ | true_ =>
-    simp only [to_nnf]
-    simp only [to_nnf_neg]
+    simp only [to_nnf_v2]
+    simp only [to_nnf_neg_v2]
     simp only [eval]
   case atom_ X | forall_ x phi ih | exists_ x phi ih =>
-    simp only [to_nnf]
-    simp only [to_nnf_neg]
+    simp only [to_nnf_v2]
+    simp only [to_nnf_neg_v2]
     simp only [eval]
   case not_ phi ih =>
-    simp only [to_nnf]
-    simp only [to_nnf_neg]
+    simp only [to_nnf_v2]
+    simp only [to_nnf_neg_v2]
     rewrite [ih]
     tauto
   case
@@ -1523,8 +1526,8 @@ theorem eval_to_nnf_neg_iff_not_eval_to_nnf
     | or_ phi psi phi_ih psi_ih
     | imp_ phi psi phi_ih psi_ih
     | iff_ phi psi phi_ih psi_ih =>
-    simp only [to_nnf]
-    simp only [to_nnf_neg]
+    simp only [to_nnf_v2]
+    simp only [to_nnf_neg_v2]
     simp only [eval]
     rewrite [phi_ih]
     rewrite [psi_ih]
@@ -1534,52 +1537,52 @@ theorem eval_to_nnf_neg_iff_not_eval_to_nnf
 example
   (V : PropValuation)
   (F : Formula_) :
-  eval V F ↔ eval V (to_nnf F) :=
+  eval V F ↔ eval V (to_nnf_v2 F) :=
   by
   induction F
   case false_ | true_ | atom_ X | forall_ x phi ih | exists_ x phi ih =>
-    unfold to_nnf
+    unfold to_nnf_v2
     rfl
   case not_ phi ih =>
-    simp only [to_nnf]
+    simp only [to_nnf_v2]
     simp only [eval]
     rewrite [ih]
-    rewrite [eval_to_nnf_neg_iff_not_eval_to_nnf V phi]
+    rewrite [eval_to_nnf_neg_iff_not_eval_to_nnf_v2 V phi]
     rfl
   case and_ phi psi phi_ih psi_ih =>
-    simp only [to_nnf]
+    simp only [to_nnf_v2]
     simp only [eval]
     rewrite [phi_ih]
     rewrite [psi_ih]
     rfl
   case or_ phi psi phi_ih psi_ih =>
-    simp only [to_nnf]
+    simp only [to_nnf_v2]
     simp only [eval]
     rewrite [phi_ih]
     rewrite [psi_ih]
     rfl
   case imp_ phi psi phi_ih psi_ih =>
-    simp only [to_nnf]
+    simp only [to_nnf_v2]
     simp only [eval]
     rewrite [phi_ih]
     rewrite [psi_ih]
-    rewrite [eval_to_nnf_neg_iff_not_eval_to_nnf V phi]
+    rewrite [eval_to_nnf_neg_iff_not_eval_to_nnf_v2 V phi]
     tauto
   case iff_ phi psi phi_ih psi_ih =>
-    simp only [to_nnf]
+    simp only [to_nnf_v2]
     simp only [eval]
     rewrite [phi_ih]
     rewrite [psi_ih]
-    rewrite [eval_to_nnf_neg_iff_not_eval_to_nnf V phi]
-    rewrite [eval_to_nnf_neg_iff_not_eval_to_nnf V psi]
+    rewrite [eval_to_nnf_neg_iff_not_eval_to_nnf_v2 V phi]
+    rewrite [eval_to_nnf_neg_iff_not_eval_to_nnf_v2 V psi]
     tauto
 
 
-lemma to_nnf_neg_is_nnf_iff_to_nnf_is_nnf
+lemma to_nnf_neg_is_nnf_iff_to_nnf_is_nnf_v2
   (F : Formula_)
   (h1 : ¬ is_subformula false_ F)
   (h2 : ¬ is_subformula true_ F) :
-  (to_nnf_neg F).is_nnf ↔ (to_nnf F).is_nnf :=
+  (to_nnf_neg_v2 F).is_nnf ↔ (to_nnf_v2 F).is_nnf :=
   by
   induction F
   case false_ =>
@@ -1589,8 +1592,8 @@ lemma to_nnf_neg_is_nnf_iff_to_nnf_is_nnf
     simp only [is_subformula] at h2
     contradiction
   case atom_ X | forall_ x phi ih | exists_ x phi ih =>
-    simp only [to_nnf]
-    simp only [to_nnf_neg]
+    simp only [to_nnf_v2]
+    simp only [to_nnf_neg_v2]
     simp only [is_nnf]
   case not_ phi ih =>
     simp only [is_subformula] at h1
@@ -1599,8 +1602,8 @@ lemma to_nnf_neg_is_nnf_iff_to_nnf_is_nnf
     simp only [is_subformula] at h2
     simp at h2
 
-    simp only [to_nnf]
-    simp only [to_nnf_neg]
+    simp only [to_nnf_v2]
+    simp only [to_nnf_neg_v2]
     rewrite [ih h1 h2]
     rfl
   case
@@ -1627,11 +1630,11 @@ example
   (h1 : F.is_prop)
   (h2 : ¬ is_proper_subformula false_ F)
   (h3 : ¬ is_proper_subformula true_ F) :
-  (to_nnf F).is_nnf :=
+  (to_nnf_v2 F).is_nnf :=
   by
   induction F
   case false_ | true_ | atom_ X =>
-    unfold to_nnf
+    unfold to_nnf_v2
     unfold is_nnf
     exact trivial
   case not_ phi ih =>
@@ -1645,8 +1648,8 @@ example
     simp only [is_subformula] at h3
     simp at h3
 
-    simp only [to_nnf]
-    rewrite [to_nnf_neg_is_nnf_iff_to_nnf_is_nnf]
+    simp only [to_nnf_v2]
+    rewrite [to_nnf_neg_is_nnf_iff_to_nnf_is_nnf_v2]
     apply ih h1
     · simp only [is_proper_subformula]
       simp
@@ -1675,7 +1678,7 @@ example
     simp only [is_proper_subformula] at psi_ih
     simp at psi_ih
 
-    simp only [to_nnf]
+    simp only [to_nnf_v2]
     simp only [is_nnf]
     tauto
   case imp_ phi psi phi_ih psi_ih =>
@@ -1695,9 +1698,9 @@ example
     simp only [is_proper_subformula] at psi_ih
     simp at psi_ih
 
-    simp only [to_nnf]
+    simp only [to_nnf_v2]
     simp only [is_nnf]
-    rewrite [to_nnf_neg_is_nnf_iff_to_nnf_is_nnf]
+    rewrite [to_nnf_neg_is_nnf_iff_to_nnf_is_nnf_v2]
     all_goals
       tauto
   case iff_ phi psi phi_ih psi_ih =>
@@ -1717,10 +1720,10 @@ example
     simp only [is_proper_subformula] at psi_ih
     simp at psi_ih
 
-    simp only [to_nnf]
+    simp only [to_nnf_v2]
     simp only [is_nnf]
-    rewrite [to_nnf_neg_is_nnf_iff_to_nnf_is_nnf]
-    rewrite [to_nnf_neg_is_nnf_iff_to_nnf_is_nnf]
+    rewrite [to_nnf_neg_is_nnf_iff_to_nnf_is_nnf_v2]
+    rewrite [to_nnf_neg_is_nnf_iff_to_nnf_is_nnf_v2]
     all_goals
       tauto
   case
